## Thu 02/18/16

### Master theorem

This theorem just tells us the the solution to the recurrences of form <br/>
T(1) = O(1) <br/>
T(n) = aT(n/b) + O(f(n)) <br/>
where f(n) = O(n<sup>2</sup>)

Ex. T(n) = 2T(n/2) + O(n) <br/>
a = 2, b = 2, c = 1<br/>
log<sub>b</sub>a = log<sub>b</sub>2 = 1


T(n) = { <br/>
  O(n<sup>log<sub>b</sub>a</sup>) if c < log<sub>b</sub>a <br/>
  O(n<sup>log<sub>b</sub>a</sup>) if c = log<sub>b</sub>a <br/>
  O(n<sup>c</sup>) if c > log<sub>b</sub>a <br/>
}

```
Ex T(n) = 2T(n/2) + O(sqrt(n) logn)
a = 2, b = 2, log(b)(a) = 1
c = 1/2 + epsilon eg. c = 2/3
sqrt(n) logn = O(n^(2/3)) => T(n) = O(n)
```

Proof: Assume f(n) <= αn<sup>2</sup> for all n>=1 <br/>
T(n) <= αT(n/b) + αn<sup>c</sup> <br/>
T(n/b) <= at(n/b<sup>2</sup>) + α(n/b)<sup>2</sup> <br/>
T(n) <=  a[aT(n/b<sup>2</sup>)] + α(n/b)<sup>c</sup>] + αn<sup>c</sup> <br/>
T(n/b<sup>2</sup>) <= aT(n/b<sup>3</sup>) + α(n/b<sup>2</sup>)<sup>c</sup> <br/>
T(n) <= a<sup>2</sup>[aT(n/b<sup>3</sup>) + α(n/b<sup>2</sup>)<sup>c</sup>] + αn<sup>c</sup>(1+a/b<sup>2</sup>) <br/>
= a<sup>3</sup>T(n/b<sup>2</sup>) + α(a<sup>2</sup>/b<sup>2c</sup>)n<sup>c</sup> + αn<sup>c</sup>(1 + a/b<sup>c</sup>) <br/>
= a<sup>3</sup>T(n/b^3) + αn^c[1 + a/b^c + (a/b^2)^2)] <br/>
= a^i T(n/b^i) + αn^c[Sum of all from j=0 to i-1 (a/b^c)^j]

n/b^i <= 1 <br/>
n <= b<sup>i</sup>
i >= log<sub>b</sub>

T(n) = n<sup>log<sub>b</sub>a</sup> + αn<sup>c</sup>[Sum of all j=0 to logn-1 (a/b<sup>c</sup>)^j]

#### Logarithmic Timeout

Log identities :

1. a<sup>log<sub>a</sub>n</sup> = n
2. log<sub>b</sub>n<sup>2</sup> = clog<sub>b</sub>n
3. log<sub>b</sub>n = log<sub>a</sub>n / log<sub>a</sub>b
4. n<sup>log<sub>b</sub>a</sup> = n<sup>log<sub>b</sub></sup>

#### Easy case :

c = log<sub>b</sub>a => a/b<sup>c</sup> = a / b <sup>log<sub>b</sub>a</sup> = 1 <br/>
T(n) <= n<sup>log<sub>b</sub>a + αn<sup>c</sup>log_b_n <br/>
 = I(n<sup>log<sub>b</sub>a</sup> log<sub>b</sub>n)
